### Detailed visual solution of the equation
 ## 1 Equation and answer
>$1x^2 + -13x + 36 = 0$  â€” The required equation.
 - First root: $(\textbf{x = 9)}$.
 - Second root: $(\textbf{x = 4)}$.
## 2 Solving
 > First, let's analyze the coefficient a, it is not equal to zero, therefore we will solve the quadratic equation. Let's calculate the discriminant!
$$D = b^2 - 4ac$$
In our case: $a = 1$ ,  $b = -13$ , $c = 36$ , hence $\Rightarrow$
 $$D = (-13)^2 - 4*1*36 = 25$$
$D > 0 \Rightarrow$ Let's calculate the roots of the quadratic equation using the formula $x_{1,2} = \frac{-b \pm \sqrt{D}}{2a}$
$$x_{1,2} = \frac{-(-13) \pm \sqrt{25}}{2 * 1}$$
>Let's write down the roots of the desired equation
$$x_1 = 9 $$ 
$$x_2 = 4 $$
>We hope that this solution was useful, thank you for using this program!
